language_formal/spark2014_semantics/nested_array_record/language.v
@@ -70,100 +70,61 @@ Inductive basic_type: Type :=
 
 Inductive type: Type := 
     | BasicT (t: basic_type)
-    | ArrayT (t: type) (l : Z) (h: Z) (* 3.6 *) (* t[l..h] *)
+    | ArrayT (t: type) (l : Z) (u: Z) (* 3.6 *) (* t[l..u] *)
     | RecordT (r: list (idnum * type)) (* 3.8 *).
-
-(*********************************************************************
-Scheme Equality for type.
-
-Lemma type_beq_complete : forall t t', t = t' -> type_beq t t' = true.
-Proof.
-  intros t t' heq.
-  subst.
-  destruct t';simpl;auto.
-Qed.
-
-Lemma type_beq_correct : forall t t', type_beq t t' = true -> t = t'.
-Proof.
-  intros t t'.
-  destruct t; destruct t';simpl;auto;intro abs; discriminate abs.
-Qed.
-
-Lemma type_beq_iff: forall t t', type_beq t t' = true <-> t = t'.
-Proof.
-  intros t t'.
-  split;intros.
-  - apply type_beq_correct. assumption.
-  - apply type_beq_complete. assumption.
-Qed.
-
-Hint Rewrite type_beq_iff: rewtype.
-Hint Rewrite type_beq_iff: rewtype_rev.
-
-Lemma type_beq_refl : forall t, type_beq t t = true.
-Proof.
-  intros t.
-  destruct t;simpl;reflexivity.
-Qed.
-*********************************************************************)
 
 (** ** Literals *)
 Inductive literal: Type :=
-	| Integer_Literal: Z -> literal (* 2.4 *)
-        | Boolean_Literal: bool -> literal (* 3.5.3 *).
+    | Integer_Literal: Z -> literal (* 2.4 *)
+    | Boolean_Literal: bool -> literal (* 3.5.3 *).
 
 (** unary and binary operators *)
 Inductive unary_operator: Type := 
-        | Not: unary_operator     
-        | Unary_Plus: unary_operator.
-(*	| Unary_Minus: unary_operator. *)
+    | Not: unary_operator     
+    | Unary_Plus: unary_operator.
+(*  | Unary_Minus: unary_operator. *)
 
 Inductive binary_operator: Type := 
-	| Equal: binary_operator 
-	| Not_Equal: binary_operator
-	| Greater_Than: binary_operator
-	| Greater_Than_Or_Equal: binary_operator
-	| Less_Than: binary_operator
-	| Less_Than_Or_Equal: binary_operator
-	| And: binary_operator
-	| Or: binary_operator
-	| Plus: binary_operator
-	| Minus: binary_operator
-	| Multiply: binary_operator
-	| Divide: binary_operator.
+    | Equal: binary_operator 
+    | Not_Equal: binary_operator
+    | Greater_Than: binary_operator
+    | Greater_Than_Or_Equal: binary_operator
+    | Less_Than: binary_operator
+    | Less_Than_Or_Equal: binary_operator
+    | And: binary_operator
+    | Or: binary_operator
+    | Plus: binary_operator
+    | Minus: binary_operator
+    | Multiply: binary_operator
+    | Divide: binary_operator.
 
 (* Ada 2012 RM, Chapter 3. Declaration and Types *)
 
 (** ** Expressions *)
 (* Chapter 4 *)
 Inductive expression: Type := 
-	| E_Literal: astnum -> literal -> expression (* 4.2 *)
-	| E_Binary_Operation: astnum -> binary_operator -> expression -> expression -> expression (* 4.5.3 and 4.5.5 *)
-	| E_Unary_Operation: astnum -> unary_operator -> expression -> expression (* 4.5.4 *) 
-        (* variable/indexed/selected component *)
-        | E_Name: astnum -> name -> expression (* 4.1 *)
-        (* array/record *) 
-        | E_Named_Record_Aggregate: astnum -> list (idnum * expression) -> expression (* 4.3.1 *) 
-        | E_Positional_Array_Aggregate: astnum -> list expression -> expression (* 4.3.3 *)
-(*      (* other forms of array/record *)
-        | E_Positional_Record_Aggregate: astnum -> list expression -> expression (* 4.3.1 *) 
-        | E_Named_Array_Aggregate: astnum -> list ((list expression (* or Range *)) * expression) -> expression (* 4.3.3 *)
-        | E_Positional_Array_Aggregate_With_Others: astnum -> list expression ->  (* others *) option expression -> expression (* 4.3.3 *) *)
+    | E_Literal: astnum -> literal -> expression (* 4.2 *)
+    | E_Name: astnum -> name -> expression (* 4.1 *)
+    | E_Binary_Operation: astnum -> binary_operator -> expression -> expression -> expression (* 4.5.3 and 4.5.5 *)
+    | E_Unary_Operation: astnum -> unary_operator -> expression -> expression (* 4.5.4 *) 
+    (* array/record *) 
+    | E_Positional_Array_Aggregate: astnum -> list expression -> expression (* 4.3.3 *)
+    | E_Named_Record_Aggregate: astnum -> list ((astnum * idnum) * expression) -> expression (* 4.3.1 *) 
 
 with name: Type := (* 4.1 *)
-        | E_Identifier: idnum -> name (* 4.1 *)
-        | E_Indexed_Component: name -> list expression -> name (* 4.1.1 *)
-        | E_Selected_Component: name -> idnum -> name          (* 4.1.3 *).
+    | E_Identifier: astnum -> idnum -> name (* 4.1 *)
+    | E_Indexed_Component: astnum -> astnum -> name -> list expression -> name (* 4.1.1 *)
+    | E_Selected_Component: astnum -> astnum -> name -> idnum -> name (* 4.1.3 *).
 
 (** ** Statements *)
 (* Chapter 5 *)
 (* Sequence is not a statement in Ada, it's a shortcut for now *)
 Inductive statement: Type := 
-	| S_Assignment: astnum -> name -> expression -> statement (* 5.2 *)
-	| S_If: astnum -> expression -> statement -> statement (* 5.3 *)
-	| S_While_Loop: astnum -> expression -> statement -> statement (* 5.5 *)
-	| S_Sequence: astnum -> statement -> statement -> statement (* 5.1 *)
-        | S_ProcCall: astnum -> procnum -> list expression -> statement.
+    | S_Assignment: astnum -> name -> expression -> statement (* 5.2 *)
+    | S_If: astnum -> expression -> statement -> statement (* 5.3 *)
+    | S_While_Loop: astnum -> expression -> statement -> statement (* 5.5 *)
+    | S_Sequence: astnum -> statement -> statement -> statement (* 5.1 *)
+    | S_ProcCall: astnum -> procnum -> list expression -> statement.
 
 (* 6.2 *)
 Inductive mode: Type := 
@@ -172,16 +133,10 @@ Inductive mode: Type :=
     | In_Out: mode.
 
 Inductive type_declaration: Type := (* 3.2.1 *)
-    (* Full_Type_Declaration *) (* 3.2.1 *)
     | Array_Type_Declaration: (* Constrained_Array_Definition, now only consider one-dimentional array *)
-        astnum -> typenum (* type name *) -> typenum -> list (expression * expression) -> type_declaration (* 3.6 *)
+        astnum -> typenum (* type name *) -> typenum -> expression -> expression -> type_declaration (* 3.6 *)
     | Record_Type_Declaration: 
         astnum -> typenum (* type name *) -> list (idnum * typenum) -> type_declaration (* 3.8 *).
-(*  | Unconstrained_Array_Type_Declaration
-    | Null_Record_Declaration: astnum -> type_declaration. (* 3.8 *)
-    | Other_Full_Type_Definition
-    | private_type_declaration (* 3.2.1 *) *)
-
 
 (* 3.3.1 *)
 Record object_declaration: Type := mkobject_declaration{
@@ -210,9 +165,9 @@ Record aspect_specification: Type := mkaspect_specification{
 (* Mutual records/inductives are not allowed in coq, so we build a record by hand. *)
 Inductive declaration: Type :=  (* 3.1 *)
     | D_Object_Declaration: astnum -> object_declaration -> declaration (* 3.3.1 *) 
-    | D_Procedure_Declaration: procedure_declaration -> declaration (* 6.1 *)
-    | Type_Declaration: astnum -> type_declaration -> declaration (* 3.2.1 *)
-    | D_Sequence: declaration -> declaration -> declaration
+    | D_Procedure_Declaration: astnum -> procedure_declaration -> declaration (* 6.1 *)
+    | D_Type_Declaration: astnum -> type_declaration -> declaration (* 3.2.1 *)
+    | D_Sequence: astnum -> declaration -> declaration -> declaration
  (* | package_declaration 
     | Other_Declarations *)
 
